\documentclass[10pt]{article}
\usepackage{graphicx}
\graphicspath{ {./images/} }
\usepackage{titlesec}
\usepackage{amssymb,amsthm,amsmath,commath}
%\pagestyle{empty}
\textwidth = 7 in\textheight = 9.5 in\oddsidemargin = -.25 in\evensidemargin = -.25 in\topmargin = -.25 in\headheight = 0.0 in\headsep = 0.0 in\parskip = 0.2in\parindent = 0.0in
\newcommand{\ds}{\displaystyle}

\title{Independent Study in Differential Equations}
\date{2018\\Fall Semester}
\author{Melissa Wallace\\Math Department, Winthrop University\\Dr. Trent Kull}

\begin{document}
\maketitle
%\renewcommand{\arraystretch}{1.2}

\section{Introduction to Material}
    ``A differential equation is an equation that contains one or more derivatives of an unknown function." - W. Trench. %make sure to actually site this later.
    The purpose of this course is to provide background before entering into the the profession of teaching. By not having taken a differential equations course at Winthrop University and needing 2 credit hours, the purpose is to obtain more knowledge and preparations in order to teach Calculus one day. %will probably add to this later once things get rolling
    It has begun as a crash course version of the standard course at Winthrop and will shift into applying Linear Algebra to the course material as well.
    
    \subsection{Basic Content Introduction}
        
    
\section{First Order Equations}
    Many differential equations derived from real world situations cannot be solved, but we will approach the ones that can be solved in this course, and the ways to solve those.\\
    
    Linear equations are the simplest form of first order equations as they can be solved using variation of parameters. A first order equation is called linear if it takes on the form $$y'=p(x)y=f(x).$$ The equation is otherwise counted as non-linear. 
    
    Begin by considering equations that can solve the following problem where a function is equal to its first derivative: $$f(x)=f'(x).$$
    The solutions will take on the form: $0, e^x, 2e^x, 3e^x, \pi e^x$. Thus we arrive at a general solution to these equations being: $$f(x)=ce^x \text{ where } c\in\mathbb{R}.$$
    
    Similarly, consider the solution to an equation where a function is equal to its second derivative: $$f(x)=f''(x).$$
    One solution to this problem looks as follows:
    \begin{eqnarray*}
        f_1(x)=\sin(x)\\
        f_1'(x)=\cos(x)\\
        f_1''(x)=\sin(x)
    \end{eqnarray*}
    It works similarly for $f(x)=\cos(x)$, or $f(x)=2\sin(x)$, $f(x)=-3\cos(x)$, or even $f(x)=2\sin(x)-3\cos(x)$. Therefore, we arrive at a general solution to these equations being: $$f(x)=c_1\sin(x)+c_2\cos(x) \text{ where } c_1,c_2\in\mathbb{R}.$$
    \\
    
%is the following actually a practice problem??? check this.
    Practice: let $x'(t)=2e^{2t}-2e^{-2t}$ and $y'(t)=-10e^{-2t}+2e^{2t}$.
    
    \subsection{Separation of Variables}
        The first strategy for solving Linear First Order Equations that we will focus on is Separation of Variables. This process looks like: $$\frac{dy}{dt}=\frac{g(t)}{f(y)} \text{ with the resulting } \int{f(y)dy}=\int{g(t)dt}.$$
        Then $f(y)\frac{dy}{dt}=g(t)$ and we assume there exists an $F(y)$ such that $\frac{dF}{dy}=f(y)$.\\
        Then notice that:
        \begin{eqnarray*}
            g(t)        &=&\frac{dF}{dy}\frac{dy}{dt} \\
            \int{g(t)dt}&=&\int{\frac{dF}{dy}\frac{dy}{dt}dt}\\
            \int{g(t)dt}&=&\int{\frac{dF}{dt}dt}     \hspace{1cm}\text{by the Chain Rule.}\\
            \int{g(t)dt}&=&F[y(t)]\\
            \int{g(t)dt}&=&\int{f(y)dy}.
        \end{eqnarray*}
    
        Now for practice:
        \begin{enumerate}
            \item[1.] Solve $\frac{dy}{dx}=-\frac{x}{y}$ with the initial condition $y(1)=1$.\\
            Notice then that $g(x)=-x$ and $f(y)=y$.\\
            Then,
            \begin{eqnarray*}
                \int{ydy}&=&\int{-xdx}\\
                \frac{y^2}{2}&=&\int{-xdx}+c_1\\
                y^2&=&x^2+c_2\\
                y^2+x^2&=&c\\
                \text{Implementing the initial value:}\\
                y(1)^2+1^2&=&c\\
                1+1&=&c\\
                c&=&2\\
                \text{Thus:}\\
                x^2+y^2&=&2
            \end{eqnarray*}
    
            \item[2.] Solve $\frac{dy}{dx}=\frac{1}{(\frac{1}{y})}.$
            Notice that $g(x)=1$ and $f(y)=\frac{1}{y}$.\\
            \begin{eqnarray*}
                \int{\frac{1}{y}dy}&=&\int{1dx}\\
                e^{\ln{\mid{y}\mid}}&=&e^{x+c_1}\\
                \abs{y}&=&e^{x+c_1}\\
                \abs{y}&=&e^x e^{c_1}\\
                \abs{y}&=&e^x c_2\\
                y&=&e^x c\\
                y&=&ce^x
            \end{eqnarray*}
            
            \item[3.] Solve $\frac{dy}{dx}=2x$ with the initial condition $y(0)=4$ and the given $c=4$.\\
            \begin{eqnarray*}
                \int{\frac{dy}{dx}dx}&=&\int{2xdx}\\
                y(x)&=&x^2+c \hspace{1cm}\text{(general solution)}\\
                y(x)&=&x^2+4v\hspace{1cm}\text{(specific solution)}\\
            \end{eqnarray*}
        \end{enumerate}
    
    In general the solution for a First Order Differential Equation solved explicitly for $\frac{dy}{dx}$, $$\frac{dy}{dx}=f(y,t).$$
    
    \subsection{Applications - Cooling Problems????}
%introduce the subject here somewhere !!!
    
    $$T'(t)=-k[T(t)-R], k>0$$
    $$\text{initial conditions:  } k=1=R, T(0)=T_0$$

    \newpage
    \subsection{Direction Fields}
%include the handout before this in the binder.
    
    \begin{center}{\bf\large MATH 471\\Lab 1\\Direction Field Homework}\end{center}
        {\bf Problem 1} $y'=ty$
            \begin{center}\includegraphics[scale=0.5]{lab1p3p1.PNG}\end{center}
        {\bf Problem 2} $y'=y^2-t^2$
            \begin{center}\includegraphics[scale=0.5]{lab1p3p2.PNG}\end{center}
        {\bf Problem 3} $y'=\frac{2ty}{1+y^2}$
            \begin{center}\includegraphics[scale=0.5]{lab1p3p3.PNG}\end{center}
        {\bf Problem 4} $y'=y(2+y)(2-y)$
            \begin{center}\includegraphics[scale=0.5]{lab1p3p4.PNG}\end{center}
        {\bf Problem 5} $y'+3y=8$
            \begin{enumerate}
                \item[a)] $y'=-3y+8$ \begin{center}\includegraphics[scale=0.5]{lab1p3p5.PNG}\end{center}
                \item[b)] My conjecture for the limiting behavior as $t \rightarrow \infty$ is that $y$ will always follow the path to 2.55.
            \end{enumerate}
        {\bf Problem 6} $(1+t^2)y'+5ty=t$
            \begin{enumerate}
                \item[a)] $y'=\frac{t-5ty}{1+t^2}$ \begin{center}\includegraphics[scale=0.5]{lab1p3p6.PNG}\end{center}
                \item[b)] My conjecture for the limiting behavior as $t \rightarrow \infty$ is that $y=0.05$.
            \end{enumerate}
        {\bf Problem 7} $ty'+ty=15-y$
            \begin{enumerate}
                \item[a)] $y'=\frac{15-y-ty}{t}$ \begin{center}\includegraphics[scale=0.5]{lab1p3p7.PNG}\end{center}
                \item[b)] My conjecture for the limiting behavior as $t \rightarrow \infty$ is that $y$ will approach 1 along the path of the curve.
            \end{enumerate}
        {\bf Problem 8} $(1+t)y'=y(4-y^2)$
            \begin{enumerate}
                \item[a)] $y'=\frac{y(4-y^2)}{1+t}$ \begin{center}\includegraphics[scale=0.5]{lab1p3p8.PNG}\end{center}
                \item[b)] My conjecture for the limiting behavior as $t \rightarrow \infty$ is that unless $y$ initially starts as 0, in which case it will remain 0, then for $y<0$, then $y=-2$. For $y>0$ then $y=2$.
            \end{enumerate}
        {\bf Problem 9}
            \begin{enumerate}
                \item[1.]    \\ \begin{center}\includegraphics[scale=0.5]{lab1p3p9.PNG}\end{center}
                \item[2.] According to the direction field, it will take approximately 2 years for the concentration to reach 0.025 or $2.5\%$.
                \item[3.] The limiting concentration seems to be 0.04. It appears to take 6 years for the concentration to reach $0.036$ or $3.6\%$. 
            \end{enumerate}
        {\bf Problem 10} When adjusting the numbers to replicate the factory no longer operating while having a concentration of $3.6\%$, it will take less than a year for the concentration to fall below $2.5\%$. Approximately $0.75$ or 9 months out of a year.
            \begin{center}\includegraphics[scale=0.5]{lab1p3p10.PNG}\end{center}
    
    
    \newpage

    \subsection{Linear nth Order Differential Equations}
%provide some kind of introduction to the material here.
    
        \begin{eqnarray*}
            a_n(t)y^{(n)}(t)+a_{n-1}y^{(n-1)}(t)+ ... + a_2(t)y''(t)+a_1(t)y'(t)+a_0y(t)&=&{\^f}(t)\\
            \text{1st order:}\\
            a_1(t)y'(t)+a_0(t)y(t)&=&\^f(t)\\
            y'(t)+\frac{a_0(t)}{a_1(t)}y(t)&=&\frac{\^f(t)}{a_1(t)}\\
            y'(t)+p(t)y&=&f(t).
        \end{eqnarray*}
        Where $f(t)=0$, the solution is {\it homogeneous}. And where $f(t)\neq 0$, the solution is called {\it inhomogeneous}.
        
    \subsection{Variation of Parameters}
%use textbook to provide an introduction as to why this approach is different from separation of variables and why we would use it.
        We'll find both a homogeneous and particular solution when approaching linear nth order differential equations with the variation of parameters approach: $$y_H, y_P.$$
        \begin{eqnarray*}
            y'+p(t)y&=&f(t)=0\\
            y_H'+p(t)y_H&=&0\\
            \frac{dy_H}{dt}&=&-p(t)y_H\\
            \int{\frac{1}{y_H}dy_H}&=&-\int{p(t)dt}\\
            \ln\abs{y_H}&=&-\int{p(t)dt}+c_1\\
            \text{Thus the homogeneous solution looks like:}\\
            y_H&=&ce^{-\int{p(t)dt}}\\
            \text{Now we assume the particular solution takes on a similar form:}\\
            y_P&=&c(t)e^{-\int{p(t)dt}}\\
            \text{We must solve:} && y_P'+p(t)y_P=f(t)\\
            y_P'(t)&=&c(t)e^{-\int{p(t)dt}}[-p(t)]+c'(t)e^{-\int{p(t)dt}}\\
            -c(t)p(t)e^{-\int{p(t)dt}}+c'(t)e^{-\int{p(t)dt}}+c(t)p(t)e^{-\int{p(t)dt}}&=&f(t)\\
            c'(t)e^{-\int{p(t)dt}}&=&f(t)\\
            c'(t)&=&f(t)e^{\int{p(t)dt}}\\
            c(t)&=&\int{f(t)e^{\int{p(t)dt}}dt}\\
            \text{So,}\\
            y_P(t)&=&e^{-\int{p(t)dt}}\int{f(t)e^{\int{p(t)dt}}dt}\\
        \end{eqnarray*}
        
        Now we combine both the particular solution and the homogeneous solution using: 
        $$y(t)=y_H(t)+y_P(t).$$
        And applying: $$y_H'+p(t)y_H=0 \text{ and } y_P'+p(t)y_P=f(t).$$
        Therefore, we get:
        \begin{eqnarray*}
            y'(t)+p(t)y(t)&=&f(t)\\
            (y_H'+y_P')+p(t)(y_H+y_P)&=&f(t)\\
            y_H'+p(t)y_H+y_P'+p(t)y_P&=&f(t)
        \end{eqnarray*}
        
        Finally, the general solution for an nth order differential equation when implementing the Variation of Parameters strategy resembles:         $$y(t)&=&ce^{-\int{p(t)dt}}+e^{-\int{p(t)dt}}\int{f(t)e^{\int{p(t)dt}}dt}$$ 
        
        Practice:
        \begin{enumerate}
            \item[1.] Given that $t\in(0,\pi)$, Solve $y'+(\cot(t))y=t\csc(t)$.\\
            Begin by setting up the homogeneous equation, $y_H'+(\cot(t))y_H=0$, then isolate $y_H'$.
            \begin{eqnarray*}
                \frac{dy_H}{dx}&=&-(\cot(x))y_H\\
                \frac{dy_H}{dt}\cdot\frac{1}{y_H} &=& -\cot(t)\\
                \int{\frac{1}{y_H}dy_H} &=& \int-\cot(t)dt\\
                \ln(y_H) &=& \ln(\sin(t))^{-1})+c &\text{via Substitution.}\\
                e^{\ln(y_H)} &=& e^{\ln(\sin(t))^{-1})+c}\\
                y_H &=& \frac{c}{\sin(t)}
            \end{eqnarray*}
            Then to also introduce the particular solution, guessing that it takes on the same form as the homogeneous solution but with $c$ being a function of $t$.
            \begin{eqnarray*}
                y_P &=& \frac{c(t)}{\sin(t)}\\
                \frac{c'(t)}{\sin(t)} &=& t(\csc(t))\\
                c'(t) &=& t\csc(t)\cdot\sin(t)\\
                c(t) &=&\int t\csc(t)\cdot\sin(t)dt\\
                c(t) &=& \int t dt\\
                c(t) &=& \frac{t^2}{2}\\
                y_{P}&=& \frac{t^2}{2\sin(t)}\\
            \end{eqnarray*}
             Thus, the solution: $y(t)=\frac{c}{\sin(t)}+\frac{t^2}{2\sin(t)}$.
        
            \item[2.] Solve $ty'+5y=7t^2$, given $t>0$.\\
            Begin by dividing through by $t$ in order to simplify the problem, then moving on to the homogeneous equation first.
            \begin{eqnarray*}
                y'+\frac{5}{t}y&=&7t\\
                y_H'+\frac{5}{t}y_H&=&0\\
                y_H'&=&-\frac{5}{t}y_H\\
                \frac{y_H'}{y_H}&=&-\frac{5}{t}\\
                \frac{dy_H'}{dt}\cdot\frac{1}{y_H}&=&-\frac{5}{t}\\
                \int{\frac{1}{y_H}dy_H}&=&\int{-\frac{5}{t}dt}\\
                \ln(y_H)&=&-5\ln(t)+c_1\\
                y_H&=&e^{\ln(t^{-5})+c_1}\\
                y_H&=&c t^{-5}\\
                y_H&=&\frac{c}{t^5}\\
            \end{eqnarray*}
            Making our guess yet again,
            \begin{eqnarray*}
                y_P&=&\frac{c(t)}{t^5}\\
                y_P&=&t^{-5}c(t)\\
                y_P'&=&-5t^{-6}c(t)+t^{-5}c'(t)
            \end{eqnarray*}
            Then inserting this equation into $y_P'+\frac{5}{t}y_H=7t$ we get the following,
            \begin{eqnarray*}
                -5t^{-6}c(t)+t^{-5}c'(t)+\frac{5}{t}\cdot\frac{c(t)}{t^5}&=&7t\\
                t^{-5}c'(t)&=&7t\\
                c'(t)&=&\frac{7t}{t^{-5}}\\
                c'(t)&=&7t^6\\
                c(t)&=&t^7\\
                y_P&=&\frac{t^7}{t^5}=t^2.
            \end{eqnarray*}
        Thus, the solution is $y=\frac{c}{t^5}+t^2$.
        
        \item[3.] Solve $y'+\frac{y}{x}=xy^2$ using the substitution $z=\frac{1}{y}$ to create a linear differential equation.\\
        Therefore, $z=z[y(x)]$ and thus $\frac{dz}{dx}=\frac{dz}{dy}\cdot\frac{dy}{dx}$. Using this, we get $z'(x)=\frac{-1}{y^2}y'$. Solving this equation for $y'$ yeilds $y'=-y^2 z'(t)$. We can now use this in place of $y'$ and $y$ within the equation.
        \begin{eqnarray*}
            \int{y'dy}&=&\int{y^2 z'(t)dy}\\
        \end{eqnarray*}
%need to locate this problem and its solution.
        \end{enumerate}
        
    \subsection{Integrating Factor}
%use textbook to introduce why this approach is different from the others. what benefit does it provide, why should we use it, and when?
    Another approach to solving nth Order Differential Equations is through the method of Integrating Factors. By using the integrating factor approach, we use the same equation: $y'(t)+p(t)y(t)=f(t)$ but this time we designate a specific factor to multiply through the equation with. We will declare this factor as follows, $$\mu=e^{\int{p(t)dt}}$$.
%add a reason why we selected mu to be this.
    Therefore, $$e^{\int{p(t)dt}}y'(t)+e^{\int{p(t)dt}}p(t)y(t)=e^{\int{p(t)dt}}f(t).$$
        
    
\end{document}